iris/ProofSysMknod.v
@@ -1670,7 +1670,7 @@ Section ProofSysMknodBody.
       { iEval (rewrite HN4a0). iExact "Hbufk". }
       iIntros (CID26 Hq26 mcr ok made kk qi ss gy inum dn bm un1 Sb1 ns1)
         "%Hcscr Hcg Hown Hpc Hsbn Hsbi Hsbs Hsbb Hpriv Hbufk Hbsl
-         %Hns1 Hir %Hun1 HopS Htx Hok".
+         %Hns1 Hir %Hun1 HopS Hok".
       iEval (rewrite HN4a0) in "Hbufk".
       assert (Hpc44 : ret_pc (N4 !!! Regidx Rra : mword 64)
                       = mword_of_int (MN + 0x44)) by (rewrite HN4ra; pcw).
@@ -1733,6 +1733,16 @@ Section ProofSysMknodBody.
         iDestruct (inode_ref_short_gen_forget with "Href") as "Href".
         iDestruct (mn_esc_acc cn gfs gi cov logstart kk ltac:(lia)
                      with "Hescrows") as "#Hesc".
+        (* CREATE'S PAYOUT IS THE ARMED DESCRIPTOR (durable-disk B''-tx2):
+           the escrow parked half of the transaction's element at create's
+           own [ilock(ip)] and create handed the other half over inside the
+           bundle, so this release disarms and the whole token comes home. *)
+        iApply fupd_wp.
+        iMod (SpecIunlock.ic_disarm_tx_log ⊤ cn gfs gi cov logstart kk ss dev
+                inum gy true ltac:(solve_ndisj) with "Hesc Hivalid Hdep")
+          as "(Hivalid & Hdep & Htx)".
+        iModIntro.
+        iEval (rewrite -Hclog) in "Htx".
         destruct (Hiregb inum ltac:(lia)) as [Hibcov Hiblog].
         iDestruct (proc_priv_bare_acc gf pj pid (upd_upt V P') with "Hpriv")
           as "[Hpbare Hpback]".
@@ -1852,7 +1862,7 @@ Section ProofSysMknodBody.
         { cbn in Hns1. lia. }
         { rewrite /sys_mknod_ret. left. rewrite Ha0f. exact HP2a0. }
       + (* ---------- ARM B: create returned 0 ---------- *)
-        iDestruct "Hok" as "%Hcrz".
+        iDestruct "Hok" as "[%Hcrz Htx]".
         iApply (wp_cbeqz_taken_s_sconf (CID := CID26) (mword_of_int (MN + 0x44))
                   (mword_of_int 10 : mword 8) (Cregidx (mword_of_int 2)) Ra0
                   mcr (K - 20)%nat b
